velusmain.ml
@@ -98,7 +98,7 @@ let compile source_name filename =
   if Cerrors.check_errors() then exit 2;
   let main_node = get_main_node p in
   match Compiler.apply_partial
-          (VelusCorrectness.compile (List.rev p) main_node)
+          (VelusCorrectness.compile p main_node)
           Asmexpand.expand_program with
   | Error errmsg -> Driveraux.print_error stderr errmsg
   | OK asm ->
