ObcToClight/Generation.v
@@ -445,6 +445,7 @@ Definition translate (do_sync: bool) (main_node: ident) (prog: program): res Cli
         let f_gvar := (f, type_of_inst main_node) in
         let ins := map glob_bind m.(m_in) in
         let outs := map glob_bind m.(m_out) in
+        let prog := rev prog in
         let cs := map (translate_class prog) prog in
         let (structs, funs) := split cs in
         let main := (main_id, make_main false main_node m) in
